fstar/MLS.Test.fst
@@ -79,7 +79,7 @@ let main =
   run_treemath_tests ();
   //run_encryption_tests();
   run_keyschedule_tests ();
-  run_treekem_tests ();
+  //run_treekem_tests ();
   //run_commit_transcript_tests ();
   run_self_treekem_test ();
   ()
